src/lang/Semantics.v
@@ -5,73 +5,73 @@ Require Import Thread.
 
 Set Implicit Arguments.
 
-Module RegSet.
-  Definition t := Reg.Fun.t Const.t.
+Module RegFile.
+  Definition t := RegFun.t Const.t.
 
-  Definition empty := Reg.Fun.init Const.zero.
+  Definition empty := RegFun.init Const.zero.
 
-  Definition eval_value (rs:t) (val:Value.t): Const.t :=
+  Definition eval_value (rf:t) (val:Value.t): Const.t :=
     match val with
-    | Value.reg r => Reg.Fun.find r rs
+    | Value.reg r => RegFun.find r rf
     | Value.const c => c
     end.
 
-  Definition eval_expr (rs:t) (rhs:Instr.expr): Const.t :=
+  Definition eval_expr (rf:t) (rhs:Instr.expr): Const.t :=
     match rhs with
-    | Instr.expr_val val => eval_value rs val
-    | Instr.expr_op1 op op1 => Op1.eval op (eval_value rs op1)
-    | Instr.expr_op2 op op1 op2 => Op2.eval op (eval_value rs op1) (eval_value rs op2)
+    | Instr.expr_val val => eval_value rf val
+    | Instr.expr_op1 op op1 => Op1.eval op (eval_value rf op1)
+    | Instr.expr_op2 op op1 op2 => Op2.eval op (eval_value rf op1) (eval_value rf op2)
     end.
 
-  Inductive eval_instr: forall (rs1:t) (i:Instr.t) (e:option ThreadEvent.t) (rs2:t), Prop :=
+  Inductive eval_instr: forall (rf1:t) (i:Instr.t) (e:option ThreadEvent.t) (rf2:t), Prop :=
   | eval_load
-      rs lhs rhs ord val:
+      rf lhs rhs ord val:
       eval_instr
-        rs
+        rf
         (Instr.load lhs rhs ord)
         (Some (ThreadEvent.rw (RWEvent.read rhs val ord)))
-        (Reg.Fun.add lhs val rs)
+        (RegFun.add lhs val rf)
   | eval_store
-      rs lhs rhs ord:
+      rf lhs rhs ord:
       eval_instr
-        rs
+        rf
         (Instr.store lhs rhs ord)
-        (Some (ThreadEvent.rw (RWEvent.write lhs (eval_value rs rhs) ord)))
-        rs
+        (Some (ThreadEvent.rw (RWEvent.write lhs (eval_value rf rhs) ord)))
+        rf
   | eval_fetch_add
-      rs lhs loc addendum ord val:
+      rf lhs loc addendum ord val:
       eval_instr
-        rs
+        rf
         (Instr.fetch_add lhs loc addendum ord)
-        (Some (ThreadEvent.rw (RWEvent.update loc val (Const.add val (eval_value rs addendum)) ord)))
-        (Reg.Fun.add lhs val rs)
+        (Some (ThreadEvent.rw (RWEvent.update loc val (Const.add val (eval_value rf addendum)) ord)))
+        (RegFun.add lhs val rf)
   | eval_assign
-      rs lhs rhs:
+      rf lhs rhs:
       eval_instr
-        rs
+        rf
         (Instr.assign lhs rhs)
         None
-        (Reg.Fun.add lhs (eval_expr rs rhs) rs)
+        (RegFun.add lhs (eval_expr rf rhs) rf)
   | eval_fence
-      rs ord:
+      rf ord:
       eval_instr
-        rs
+        rf
         (Instr.fence ord)
         (Some (ThreadEvent.fence ord))
-        rs
+        rf
   | eval_syscall
-      rs lhs rhses lhs_val:
+      rf lhs rhses lhs_val:
       eval_instr
-        rs
+        rf
         (Instr.syscall lhs rhses)
-        (Some (ThreadEvent.syscall (Event.mk lhs_val (map (eval_value rs) rhses))))
-        (Reg.Fun.add lhs lhs_val rs)
+        (Some (ThreadEvent.syscall (Event.mk lhs_val (map (eval_value rf) rhses))))
+        (RegFun.add lhs lhs_val rf)
   .
-End RegSet.
+End RegFile.
 
 Module State.
   Structure t: Type := mk {
-    regs: RegSet.t;
+    regs: RegFile.t;
     stmts: list Stmt.t;
   }.
 
@@ -80,26 +80,26 @@ Module State.
 
   Inductive step: forall (s1:t) (e:option ThreadEvent.t) (s1:t), Prop :=
   | step_instr
-      rs1 i e rs2 stmts
-      (INSTR: RegSet.eval_instr rs1 i e rs2):
+      rf1 i e rf2 stmts
+      (INSTR: RegFile.eval_instr rf1 i e rf2):
       step
-        (mk rs1 ((Stmt.instr i)::stmts))
+        (mk rf1 ((Stmt.instr i)::stmts))
         e
-        (mk rs2 stmts)
+        (mk rf2 stmts)
   | step_ite
-      rs cond s1 s2 stmts:
+      rf cond s1 s2 stmts:
       step
-        (mk rs ((Stmt.ite cond s1 s2)::stmts))
+        (mk rf ((Stmt.ite cond s1 s2)::stmts))
         None
-        (mk rs ((if RegSet.eval_expr rs cond
+        (mk rf ((if RegFile.eval_expr rf cond
                  then s1
                  else s2) ++ stmts))
   | step_dowhile
-      rs s cond stmts:
+      rf s cond stmts:
       step
-        (mk rs ((Stmt.dowhile s cond)::stmts))
+        (mk rf ((Stmt.dowhile s cond)::stmts))
         None
-        (mk rs (s ++ (Stmt.ite cond ((Stmt.dowhile s cond)::nil) nil) :: stmts))
+        (mk rf (s ++ (Stmt.ite cond ((Stmt.dowhile s cond)::nil) nil) :: stmts))
   .
 End State.
 
