src/lib/Basic.v
@@ -1,0 +1,86 @@
+Require String.
+Require Import List.
+Require Import PArith.
+Require Import FMapPositive.
+Require Import FMapFacts.
+Require Import MSetList.
+
+Require Import DataStructure.
+
+Set Implicit Arguments.
+
+Module Ident <: OrderedTypeWithLeibniz.
+  Include Pos.
+
+  Lemma eq_leibniz (x y: t): eq x y -> x = y.
+  Proof. auto. Qed.
+
+  Parameter of_string: String.string -> t.
+  Hypothesis of_string_inject:
+    forall s1 s2 (H12: s1 <> s2), of_string s1 <> of_string s2.
+
+  Ltac ltb_tac :=
+    match goal with
+    | [H: compare ?x1 ?x2 = _ |- _] =>
+      generalize (compare_spec x1 x2); rewrite H; clear H;
+      intro H; inversion H; subst; clear H
+    | [H: lt ?x ?x |- _] =>
+      destruct lt_strorder; congruence
+    | [H: lt ?x ?y |- _] =>
+      rewrite H in *; clear H
+    | [H: eq ?x ?y |- _] =>
+      rewrite H in *; clear H
+    end.
+End Ident.
+
+Module IdentFun := UsualFun (Ident).
+Module IdentSet := UsualSet (Ident).
+
+Module IdentMap.
+  Include PositiveMap.
+  Module Facts := FMapFacts.Facts (PositiveMap).
+  Module Properties := FMapFacts.Properties (PositiveMap).
+
+  Definition get_max V (pred: V -> nat) (m:t V): nat :=
+    fold
+      (fun _ v res => max (pred v) res)
+      m
+      0.
+
+  Lemma get_max_spec V (pred: V -> nat) m:
+    forall i v (FIND: find i m = Some v), pred v <= get_max pred m.
+  Proof.
+    unfold find, get_max.
+    rewrite fold_1, <- fold_left_rev_right.
+    intros.
+    apply elements_correct in FIND.
+    apply in_rev in FIND.
+    revert FIND. generalize (rev (elements m)).
+    induction l; intros; inversion FIND; subst; simpl.
+    - apply Max.le_max_l.
+    - rewrite <- Max.le_max_r. apply IHl. auto.
+  Qed.
+End IdentMap.
+
+
+Definition option_eq_dec
+           A (eq_dec: forall (l r:A), {l = r} + {l <> r})
+           (l r: option A): {l = r} + {l <> r}.
+Proof.
+  refine
+    (match l, r with
+     | Some l, Some r => _
+     | None, None => _
+     | _, _ => _
+     end);
+    try (left; auto; fail);
+    try (right; congruence; fail).
+  destruct (eq_dec l r).
+  - subst. left. auto.
+  - right. contradict n. inversion n. auto.
+Defined.
+
+Notation rtc := (clos_refl_trans _). (* reflexive transitive closure *)
+Notation rc := (clos_refl _). (* reflexive transitive closure *)
+Notation tc := (clos_trans _). (* transitive closure *)
+Hint Immediate rt_step rt_refl t_step.
