src/lib/BoolOrderedType.v
@@ -1,0 +1,87 @@
+Require Import Orders.
+Require Import List.
+
+Import ListNotations.
+
+Module Type S.
+  Parameter (t:Type).
+  Parameter (eq_dec: forall (lhs rhs:t), {lhs = rhs} + {lhs <> rhs}).
+
+  Parameter (ltb: forall (lhs rhs:t), bool).
+  Parameter (ltb_trans: forall (x y z:t) (XY: ltb x y = true) (YZ: ltb y z = true), ltb x z = true).
+  Parameter (ltb_irrefl: forall x, ltb x x = false).
+  Parameter (ltb_eq: forall (lhs rhs:t) (LR: ltb lhs rhs = false) (RL: ltb rhs lhs = false), lhs = rhs).
+End S.
+
+Module Make (O:S).
+  Definition eq := @eq O.t.
+  Program Instance eq_equiv: Equivalence eq.
+  Lemma eq_leibniz (x y: O.t): eq x y -> x = y.
+  Proof. auto. Qed.
+
+  Definition lt (lhs rhs:O.t): Prop := O.ltb lhs rhs = true.
+
+  Program Instance lt_strorder: StrictOrder lt.
+  Next Obligation.
+    repeat intro. unfold lt in H.
+    rewrite O.ltb_irrefl in H. congruence.
+  Qed.
+  Next Obligation.
+    repeat intro. unfold lt in *.
+    apply O.ltb_trans with y; auto.
+  Qed.
+
+  Lemma lt_compat : Proper (eq ==> eq ==> iff) lt.
+  Proof.
+    repeat intro. unfold eq in *. subst. constructor; auto.
+  Qed.
+
+  Definition compare (lhs rhs:O.t): comparison :=
+    if O.ltb lhs rhs
+    then Lt
+    else if O.ltb rhs lhs
+         then Gt
+         else Eq.
+
+  Lemma compare_spec (x y: O.t):
+    CompareSpec (eq x y) (lt x y) (lt y x) (compare x y).
+  Proof.
+    unfold lt, compare.
+    destruct (O.ltb x y) eqn:XY.
+    { constructor. auto. }
+    destruct (O.ltb y x) eqn:YX.
+    { constructor. auto. }
+    constructor. apply O.ltb_eq; auto.
+  Qed.
+
+  Ltac ltb_tac :=
+    match goal with
+    | [H: compare ?x1 ?x2 = _ |- _] =>
+      generalize (compare_spec x1 x2); rewrite H; clear H;
+      intro H; inversion H; subst; clear H
+    | [H: lt ?x ?x |- _] =>
+      destruct lt_strorder; congruence
+    | [H: lt ?x ?y |- _] =>
+      rewrite H in *; clear H
+    | [H: eq ?x ?y |- _] =>
+      rewrite H in *; clear H
+    end.
+End Make.
+
+Fixpoint compose_comparisons (l: list comparison): bool :=
+  match l with
+  | nil => false
+  | Lt::_ => true
+  | Gt::_ => false
+  | Eq::l => compose_comparisons l
+  end.
+
+Ltac ltb_des :=
+  match goal with
+  | [H: context[match ?c with | Eq => _ | Lt => _ | Gt => _ end] |- _] =>
+    let COND := fresh "COND" in
+    destruct c eqn:COND
+  | [|- context[match ?c with | Eq => _ | Lt => _ | Gt => _ end]] =>
+    let COND := fresh "COND" in
+    destruct c eqn:COND
+  end.
