src/lib/DataStructure.v
@@ -1,0 +1,95 @@
+Require Import Equalities.
+Require Import FunctionalExtensionality.
+Require Import MSetList.
+Require Import MSetFacts.
+
+Require Import sflib.
+
+Set Implicit Arguments.
+
+Module UsualFun (A:UsualDecidableType).
+  Section UsualFun.
+    Variable (B:Type).
+
+    Definition t := forall (a:A.t), B.
+
+    Definition init (b:B): t := fun _ => b.
+
+    Definition find (a:A.t) (f:t): B := f a.
+
+    Definition add (a:A.t) (b:B) (f:t): t :=
+      fun a' =>
+        if A.eq_dec a' a
+        then b
+        else find a' f.
+
+    Definition init_spec a b:
+      find a (init b) = b.
+    Proof. auto. Qed.
+
+    Definition add_spec a' a b f:
+      find a' (add a b f) =
+      if A.eq_dec a' a
+      then b
+      else find a' f.
+    Proof. auto. Qed.
+
+    Lemma add_twice a1 a2 b1 b2 f
+          (DIFF: a1 <> a2):
+      add a1 b1 (add a2 b2 f) = add a2 b2 (add a1 b1 f).
+    Proof.
+      extensionality i. unfold add, find.
+      destruct (A.eq_dec i a1), (A.eq_dec i a2); auto.
+      congruence.
+    Qed.
+  End UsualFun.
+End UsualFun.
+
+
+Module UsualSet (S: OrderedTypeWithLeibniz).
+  Module Self := MSetList.MakeWithLeibniz (S).
+  Module Facts := MSetFacts.Facts (Self).
+  Include Self.
+
+  Definition disjoint (lhs rhs:t): Prop :=
+    forall s, <<DISJ: mem s lhs && mem s rhs = false>>.
+
+  Inductive disjoint_add lhs a rhs: Prop :=
+  | disjoint_add_intro
+      (DISJ: disjoint lhs (singleton a))
+      (ADD: add a lhs = rhs)
+  .
+
+  Lemma ext lhs rhs
+        (EXT: forall i, mem i lhs = mem i rhs):
+    lhs = rhs.
+  Proof.
+    apply eq_leibniz. intro i.
+    rewrite ? Facts.mem_iff. rewrite EXT.
+    constructor; auto.
+  Qed.
+
+  Lemma disjoint_spec lhs rhs
+        (DISJ: disjoint lhs rhs):
+    lhs = diff (union lhs rhs) rhs.
+  Proof.
+    apply eq_leibniz. intro i. specialize (DISJ i).
+    rewrite ? Facts.mem_iff.
+    rewrite Facts.diff_b, Facts.union_b.
+    destruct (mem i lhs), (mem i rhs); simpl in *;
+      constructor; intro; auto.
+  Qed.
+
+  Lemma disjoint_add_spec lhs a rhs
+        (DISJ: disjoint_add lhs a rhs):
+    lhs = remove a rhs.
+  Proof.
+    apply eq_leibniz. intro i.
+    inversion DISJ. subst. clear DISJ. specialize (DISJ0 i).
+    rewrite ? Facts.mem_iff.
+    rewrite Facts.singleton_b, Facts.remove_b, Facts.add_b in *.
+    rewrite andb_true_iff in *.
+    destruct (Facts.eqb a i); simpl in *; intuition.
+    rewrite H in DISJ0. auto.
+  Qed.
+End UsualSet.
